Full restructuring of the formalisation. Converted from unbounded games to bounded games and re-proved the previous lemmas.

theories/algebra/NR_PRF.ec
@@ -1,93 +1,194 @@
 (* NR-PRF *)
 require import Int Real List SmtMap Distr DList FSet.
-require (*--*) GroupAction PRF.
+require (*--*) GroupAction.
 
+(* We need a regular, effective, abelian group action for this construction *) 
 clone import GroupAction.ARegEGA as Ega.
-
-(*
-(* Could be MUniform here *)
-op dR : { set distr | is_lossless dR } as dR_ll.
-*)
-clone import MFinite as DR with
-    type t <- set.
-op dR = DR.dunifin.
 
 (* Setup keyspace, domain, and range *)
 type K = group * group.
 type D = bool. (* Only one bit for the moment but will be an l-bit word *) 
 type R = set.
 
-clone import PRF as PRF_t with
-    type D <- D, 
-    type R <- R.
-    
-clone import RF with
-    op dR <- fun _=> dR
-proof
-    dR_ll by (move=> _; exact: DR.dunifin_ll).
-
+(* This is the construction we wish to prove is a PRF *)
 op F (k : K) (m : D) =
     if   m
     then act (k.`1 * k.`2) x0
     else act k.`1 x0.
 
-clone import PseudoRF as Prf with
-    type K  <- K,
-      op F  <- F,
-      op dK <- sample `*` sample
-proof *.
-realize dK_ll.
-apply: dprod_ll.
-search is_lossless.
-split.
-+ exact DG.dunifin_ll.
-exact DG.dunifin_ll.
+(* Setup the uniform distribution on our range *)
+clone import MFinite as DR with
+    type t <- R.
+op dR : D -> R distr = fun _ => DR.dunifin.
+lemma dR_ll (x : D) : is_lossless (dR x).
+proof.
+exact DR.dunifin_ll.
+qed. 
+
+op dK : K distr = sample `*` sample.
+lemma dK_ll : is_lossless dK.
+proof.
+apply dprod_ll.
+split; exact DG.dunifin_ll.
 qed.
 
-(* Lemma 4.21 *)
-(* Start by just considering the case when l = 1, here we will just have two games for an adversary to distinguish *)
+(* ------------------------------------------------------ *)
+(* Setup the bounded PRF games/oracles/adversaries *)
 
-(* This adversary attempts to distinguish between the following two games *)
-module type WPR_Oracles = {
-    proc doit(_ : D): R
+module type Bounded_PRF = {
+    proc init(Q : int) : unit
+    proc f(_ : D) : R
 }.
 
-module type Adversary1 (O : WPR_Oracles) = {
+module type PRF_Oracles = {
+    proc f(_ : D) : R
+}.
+
+module type Distinguisher (F : PRF_Oracles) = {
     proc distinguish() : bool
 }.
 
-(* Real PRF *)
-module Hybrid0 (A : Adversary1) = {
-    var g0, g1 : Ega.group
-
-    module O = {
-        (** var c : int **)
-        proc doit(s) = {
-            var yq;
-(** if c < Q, doit and increment c, otherwise, do nothing, return witness **)
-            yq <- act g0 x0;
-            if (s) {
-                yq <- act g1 yq;
-            }
-            return yq;
-        }
-    }
-
-    proc main () : bool = {
-        var b : bool;
-
-        (* Sample the key *)
-        g0 <$ sample;
-        g1 <$ sample;
-        (** c <- 0; **)
-
-        (* Allow the adversary to make Q adaptive queries *)
-        b <@ A(O).distinguish();
+module Bounded_PRF_IND (F : Bounded_PRF) (D : Distinguisher) = {
+    proc main(Q : int) : bool = {
+        var b;
+        F.init(Q);
+        b <@ D(F).distinguish();
         return b;
     }
 }.
 
-module (A (D : Distinguisher) : Adversary1) (F : WPR_Oracles) = {
+module Bounded_PRF_Real = {
+    var k : K
+    var c, q : int
+    
+    proc init(Q : int) : unit = {
+        k <$ dK;
+        q <- Q;
+        c <- 1;
+    }
+
+    proc f(x : D) : R = {
+        var val : R;
+        if (c <= q) {
+            val <- F k x;
+            c <- c + 1;
+        } else {
+            val <- witness;
+        }        
+        return val;
+    }
+}.
+
+module Bounded_PRF_Ideal = {
+    var c, q : int
+    var m : (D, R) fmap
+
+    proc init(Q : int): unit = {
+        q <- Q;
+        c <- 1;
+        m <- empty;
+    }
+
+    proc f(x : D) : R = {
+        var val : R;
+        if (c <= q) {
+            if (x \notin m) {
+                val <$ dR x;
+                m.[x] <- val;
+            }
+            val <- (oget m.[x]);
+            c <- c + 1;
+        } else {
+            val <- witness;
+        }
+        return val;
+    }
+}.
+
+(* ------------------------------------------------------------ *)
+(* Lemma 4.21 *)
+(* Start by just considering the case when l = 1, here we will just have two games for an adversary to distinguish *)
+
+module type Hybrid_PRF = {
+    proc init(_ : int) : unit
+    proc doit(_ : D) : R
+}.
+
+module type WPR_Oracles = {
+    proc doit(_ : D) : R
+}.
+
+module type Hybrid_PRF_Adv (O : WPR_Oracles) = {
+    proc distinguish() : bool
+}.
+
+module Hybrid_PRF_IND (H : Hybrid_PRF) (A : Hybrid_PRF_Adv) = {
+    proc main (Q : int) : bool = {
+        var b : bool;
+        H.init(Q);
+        b <@ A(H).distinguish();
+        return b;
+    }
+}.
+
+module Hybrid_PRF_0 = {
+    var g0, g1 : group
+    var c, q : int
+
+    proc init(Q : int) = {
+        g0 <$ sample;
+        g1 <$ sample;
+        q <- Q;
+        c <- 1;
+    }
+
+    proc doit(s) = {
+        var val;
+
+        (* Make sure we can't make more than Q, 'proper', queries *)
+        if (c <= q) {
+            val <- act g0 x0;
+            if (s) {
+                val <- act g1 val;
+            }
+            c <- c + 1;
+        } else {
+            val <- witness;
+        }
+        return val;
+    }
+}.
+
+module Hybrid_PRF_L = {
+    var m : (D, R) fmap
+    var q, c : int
+  
+    proc init(Q : int) = {
+        q <- Q;
+        c <- 1;
+        m <- empty;
+    }
+
+    proc doit(s) = {
+        var gq, val;
+        if (c <= q) {
+            if (s \notin m) {
+                gq <$ sample;
+                val <- act gq x0;
+                m.[s] <- val;
+            } else {
+                val <- oget m.[s];
+            }
+            c <- c + 1;
+        } else {
+            val <- witness;
+        }
+        return val;
+    }
+}.
+
+(* Simply wrap around the distinguisher for a PRF *)
+module (A (D : Distinguisher) : Hybrid_PRF_Adv) (F : WPR_Oracles) = {
     module O = {
         proc f = F.doit
     }
@@ -102,213 +203,210 @@ module (A (D : Distinguisher) : Adversary1) (F : WPR_Oracles) = {
 
 (** |Pr[IND(PRF, D).main() @ &m: res] - Pr[IND(RF, D).main() @ &m: res]|
     <= Advantage of A(D) against something we think is hard **)
+
 require (*--*) DProd.
 clone DProd.ProdSampling with
   type t1 <- group,
   type t2 <- group.
 
-lemma Hybrid0_INDPRF_eq (D <: Distinguisher {Hybrid0, PRF} ) &m:
-  Pr[IND(PRF, D).main() @ &m: res] = Pr[Hybrid0(A(D)).main() @ &m: res].
+lemma Hybrid_PRF_0_PRF_Real_eq (D <: Distinguisher {Hybrid_PRF_0, Bounded_PRF_Real}) (x : int) &m:
+  Pr[Bounded_PRF_IND(Bounded_PRF_Real, D).main(x) @ &m: res] = Pr[Hybrid_PRF_IND(Hybrid_PRF_0, A(D)).main(x) @ &m: res].
 proof.
 byequiv=> //.
 proc.
 inline *.
-seq  1  2: (={glob D} /\ PRF.k{1} = (Hybrid0.g0,Hybrid0.g1){2}).
+sp.
+seq  1  2: (={glob D}
+            /\ Bounded_PRF_Real.k{1} = (Hybrid_PRF_0.g0,Hybrid_PRF_0.g1){2}
+            /\ ={Q}
+            /\ ={Q0}
+            ).
 + conseq />.
   transitivity {1} (** Which memory should the piece of code operate in? **)
-               { PRF.k <@ ProdSampling.S.sample(sample, sample); } (** Which piece of code? **)
-               (true ==> ={PRF.k}) (** Left-to-step similarity **)
-               (true ==> PRF.k{1} = (Hybrid0.g0, Hybrid0.g1){2}) (** Step-to-right similarity **)=> //.
+               { Bounded_PRF_Real.k <@ ProdSampling.S.sample(sample, sample); } (** Which piece of code? **)
+               (true ==> ={Bounded_PRF_Real.k}) (** Left-to-step similarity **)
+               (true ==> Bounded_PRF_Real.k{1} = (Hybrid_PRF_0.g0, Hybrid_PRF_0.g1){2}) (** Step-to-right similarity **)=> //.
   + by inline {2} 1; auto.
   transitivity {2}
-               { (Hybrid0.g0, Hybrid0.g1) <@ ProdSampling.S.sample2(sample, sample); }
-               ( true ==> PRF.k{1} = (Hybrid0.g0, Hybrid0.g1){2})
-               (true ==> ={Hybrid0.g0, Hybrid0.g1})=> //.
+               { (Hybrid_PRF_0.g0, Hybrid_PRF_0.g1) <@ ProdSampling.S.sample2(sample, sample); }
+               ( true ==> Bounded_PRF_Real.k{1} = (Hybrid_PRF_0.g0, Hybrid_PRF_0.g1){2})
+               (true ==> ={Hybrid_PRF_0.g0, Hybrid_PRF_0.g1})=> //.
   + by call ProdSampling.sample_sample2; auto=> /> [].
   by inline {1} 1; auto.
 wp.
-call (: PRF.k{1} = (Hybrid0.g0,Hybrid0.g1){2}).
+sp.
+call (: Bounded_PRF_Real.k{1} = (Hybrid_PRF_0.g0, Hybrid_PRF_0.g1){2}
+      /\ Bounded_PRF_Real.c{1} = Hybrid_PRF_0.c{2}
+      /\ Bounded_PRF_Real.q{1} = Hybrid_PRF_0.q{2}
+      ).
 + proc; wp; skip=> />.
-  move=> &2 _ @/F /=.
+  move=> &2 _ _ @/F /=.  
   rewrite comp.
-  exact actC.  
-by skip.
+  exact: actC.
+skip=> />.
 qed.
 
-(* Ideal Randomness *)
-module Hybrid1 (A : Adversary1) = {
-    (* Keep track of previous input output pairs *) 
-    var queries : (D, R) fmap
-
-    module O = {
-        proc doit(s) = {
-            var gq, yq;
-            
-            if (s \notin queries) {
-                gq <$ sample;
-                yq <- act gq x0;
-                queries.[s] <- yq;
-            } else {
-                yq <- oget queries.[s];
-            }
-            return yq;
-        }
-    }
-
-    proc main () : bool = {
-        var b : bool;
-        queries <- empty;
-        b <@ A(O).distinguish();
-        return b;
-    }
-}.
-
-lemma Hybrid1_INDRF_eq (D <: Distinguisher {Hybrid1, RF} ) &m:
-    Pr[IND(RF, D).main() @ &m: res] = Pr[Hybrid1(A(D)).main() @ &m: res].
+lemma Hybrid_PRF_L_PRF_Real_eq (D <: Distinguisher {Hybrid_PRF_L, Bounded_PRF_Ideal}) (a : int) &m:
+    Pr[Bounded_PRF_IND(Bounded_PRF_Ideal, D).main(a) @ &m: res] = Pr[Hybrid_PRF_IND(Hybrid_PRF_L, A(D)).main(a) @ &m: res].
 proof.
 byequiv=> //.
 proc.
 inline *.
 wp.
-call (: RF.m{1} = Hybrid1.queries{2}). (* maps are equivalently distributed *)
+sp.
+call (:  Bounded_PRF_Ideal.m{1} = Hybrid_PRF_L.m{2}
+      /\ Bounded_PRF_Ideal.c{1} = Hybrid_PRF_L.c{2}
+      /\ Bounded_PRF_Ideal.q{1} = Hybrid_PRF_L.q{2}
+      ).
 + proc.
   if.
-  + move=> &1 &2.
-    case=> h1 h2.
-    by subst.
-  + seq 1 2 : (x{1} = s{2} /\ RF.m{1} = Hybrid1.queries{2} /\ r{1} = yq{2}).
-    + wp.
-      rnd (fun x => extract x0 x) (fun g => act g x0).
-      skip=> />.
-      move=> &2 _.
-      split.
-      + move=> g _.
-        exact extractUniq.
-      move=> _.
-      split.
-      + move=> g _.
-        have /= <- := dmap1E_can dR (extract x0) (fun g=> act g x0) g _ _.
-        + by rewrite /cancel=> g'; rewrite -extractUniq.
-        + by move=> x _ /=; rewrite extractP.
-        congr; apply: eq_funi_ll.
-        + exact: DG.dunifin_funi.
-        + exact: DG.dunifin_ll.
-        + apply/dmap_funi.
-          + exists (fun g=> act g x0); split.
-            + by move=> x; exact: extractP.
-            by move=> h; rewrite -extractUniq.
-          exact: dunifin_funi.
-        exact/dmap_ll/dunifin_ll.
-      move=> _ r rin.
-      by rewrite extractP.
-    wp.
-    skip.
-    move=> &1 &2.
-    case=> eq1.
-    case=> eq2 eq3.
-    simplify.
-    subst.
-    split.
-    + rewrite get_set_sameE.
+  + by move=> />.
+  + if.
+    + by move=> />.
+    + seq 1 2 : (x{1} = s{2}
+                /\ ={val}
+                /\ Bounded_PRF_Ideal.m{1} = Hybrid_PRF_L.m{2}
+                /\ Bounded_PRF_Ideal.c{1} = Hybrid_PRF_L.c{2}
+                /\ Bounded_PRF_Ideal.q{1} = Hybrid_PRF_L.q{2}
+                ).
+      + wp.
+        rnd (fun x => extract x0 x) (fun g => act g x0).
+        skip=> &1 &2.
+        do case => eq1 eq2 _ _ />.
+        split.
+        + move=> g _.
+          exact extractUniq.
+        move=> _.
+        split.
+        + move=> g _.
+          have /= <- := dmap1E_can DR.dunifin (extract x0) (fun g=> act g x0) g _ _.
+            + by rewrite /cancel=> g'; rewrite -extractUniq.
+            + by move=> x _ /=; rewrite extractP.
+          congr; apply: eq_funi_ll.
+          + exact: DG.dunifin_funi.
+          + exact: DG.dunifin_ll.
+          + apply/dmap_funi.
+            + exists (fun g=> act g x0); split.
+              + by move=> x; exact: extractP.
+              by move=> h; rewrite -extractUniq.
+            exact: dunifin_funi.
+          exact/dmap_ll/dunifin_ll.
+        move=> _ r rin.
+        by rewrite extractP.
+      wp.
+      skip.
+      move=> &1 &2 />.
+      rewrite get_set_sameE.
       trivial.
-    trivial.
+    wp.
+    by skip.
   wp.
   by skip.
-wp.
 by skip.
 qed.
 
 (* ----------------------------------------------- *)
-(* Lemma 4.20 *)
-module type Adversary2 = {
-    proc solve(x0 : set, ins : (set * set) list, Q : int) : bool
+module type Hybrid_WPR = {
+    proc init(_ : int) : unit
+    proc vals() : R * R
 }.
 
-module GameReal (A : Adversary2) = {
-    proc main (Q : int) : bool = {
-        var gt : group;
-        var gs : group list;
-        var xs : (set * set) list;
+module type H_WPR_Oracles = {
+    proc vals() : R * R
+}.
+
+module type Hybrid_WPR_Adv (F : H_WPR_Oracles) = {
+    proc solve() : bool
+}.
+
+module Hybrid_WPR_IND (H : Hybrid_WPR) (A : Hybrid_WPR_Adv) = {
+    proc main(Q : int) : bool = {
         var b : bool;
-        
-        gt <$ sample;
-        gs <$ dlist sample Q;
-        xs <- map (fun (g : group) => (act g x0, act gt (act g x0))) gs;
-        b <@ A.solve(x0, xs, Q);
+        H.init(Q);
+        b <@ A(H).solve();
         return b;
     }
 }.
 
-module GameIdeal (A : Adversary2) = {
-    proc main (Q : int) : bool = {
-        var gs : group list;
-        var hs : group list;
-        var ts : (group * group) list;
-        var b : bool;
-        var xs : (set * set) list;
-        
-        gs <$ dlist sample Q;
-        hs <$ dlist sample Q;
-        ts <- zip gs hs;
-        xs <- map (fun (t : group * group) => (act (t.`1) x0, act (t.`2) (act (t.`1) x0))) ts;
-        b <- A.solve(x0, xs, Q);
-        return b;
-    }
-}.
-
-
-module (Adv (A : Adversary1) : Adversary2) = {
-    var queries : (bool, (set * set)) fmap
-    var cnt, q : int
-    var els : (set * set) list
+module Hybrid_WPR_Ideal = {
+    var q, c : int
+    var gt : group
   
-    module O = {
-        proc doit(s) : set = {
-            var xq, yq : set;
-            
-            if (q <= cnt) {
-                cnt <- 1;
-            }
-
-            if (s \notin queries) {
-                (xq, yq) <- (oget (onth els cnt));
-                cnt <- cnt + 1;
-                queries.[s] <- (xq, yq);
-            } else {
-                (xq, yq) <- (oget queries.[s]);
-            }
-          
-            (* FIXME: why doesn't this work
-            if (s) {
-                return yq;
-            } else {
-                return xq;
-            }
-            *)
-
-            return s ? yq : xq;
-        }  
-    }
-  
-    proc solve(x0 : set, ins : (set * set) list, Q : int) = {
-        var s, b : bool;
-        var xq, yq : set;
-        
-        els <- ins;
+    proc init(Q : int) = {
         q <- Q;
-        cnt <- 1;
-        b <@ A(O).distinguish();
+        c <- 1;
+        gt <$ sample;
+    }
+
+    proc vals() = {
+        var gq, xq, yq;
+        if (c <= q) {
+            gq <$ sample;
+            xq <- act gq x0;
+            yq <- act gt xq;
+            c <- c + 1;
+        } else {
+            (xq, yq) <- witness;
+        }
+        return (xq, yq);
+    }
+}.
+
+module Hybrid_WPR_Real = {
+    var q, c : int
+  
+    proc init(Q : int) = {
+        q <- Q;
+        c <- 1;
+    }
+
+    proc vals() = {
+        var gq, hq, xq, yq;
+        if (c <= q) {
+            gq <$ sample;
+            hq <$ sample;
+            xq <- act gq x0;
+            yq <- act hq xq;
+            c <- c + 1;
+        } else {
+            (xq, yq) <- witness;
+        }
+        return (xq, yq);
+    }
+}.
+
+module (B (D : Hybrid_PRF_Adv) : Hybrid_WPR_Adv) (F : H_WPR_Oracles) = {
+    module O = {
+        var m : (D, R) fmap
+      
+        proc doit(s : D) = {
+            var val : R;
+            var tup : R * R;
+            if (s \notin m) {
+                tup <- F.vals();
+                if (s) {
+                    val <- tup.`1;            
+                } else {
+                    val <- tup.`2; 
+                }
+                m.[s] <- val;
+            } else {
+                val <- oget m.[s];
+            }
+            return val;
+        }
+    }  
+
+    proc solve() = {
+        var b;
+        b <@ D(O).distinguish();
         return b;
     }
 }.
 
-lemma Lem20_IND_eq_Real (A <: Adversary1 {GameIdeal, GameReal}) (Q : int) &m:
-  (** Hybrid 0 and GameReal need to actively bound number of oracle queries **)
-  Pr[Hybrid0(A).main() @ &m: res] = Pr[GameReal(Adv(A)).main(Q) @ &m: res].
+
+lemma Hybrid_WPR_Real_Hybrid_PRF_0_eq (A <: Hybrid_PRF_Adv{Hybrid_WPR_Real, Hybrid_PRF_0}) (x : int) &m:
+  Pr[Hybrid_PRF_IND(Hybrid_PRF_0, A).main(x) @ &m: res] = Pr[Hybrid_WPR_IND(Hybrid_WPR_Real, B(A)).main(x) @ &m: res].
 proof.
-byequiv=> //.
-proc.
-inline *.
-wp.
 admit.
 qed.
